{
  "@context": {
    "dcterms": "http://purl.org/dc/terms/",
    "owl": "http://www.w3.org/2002/07/owl#",
    "rdf": "http://www.w3.org/1999/02/22-rdf-syntax-ns#",
    "rdfs": "http://www.w3.org/2000/01/rdf-schema#",
    "schema": "https://schema.org/",
    "sh": "http://www.w3.org/ns/shacl#",
    "skos": "http://www.w3.org/2004/02/skos/core#",
    "xsd": "http://www.w3.org/2001/XMLSchema#",
	"vcdm": "https://www.w3.org/ns/credentials/v2/",
	"aiao": "https://w3id.org/aiao/",
	"impact": "https://w3id.org/impactont/",
	"claim": "https://w3id.org/claimont/",
	"infocomm": "https://w3id.org/infocomm/",
	"data": "https://jellyfiiish.xyz/ns/",
	"indimp": "https://independentimpact.org/ns/",
	"hed": "https://independentimpact.org/ns/hedera/"
  },
  "@graph": [
	{
      "@id": "indimp:PlatformUser",
	  "@type": "rdfs:Class",
	  "skos:definition": "An actor on the Independent Impact platform.",
      "rdfs:label": "PlatformUser",
      "rdfs:subClassOf": {
        "@id": "owl:Thing"
      }
    },	
	{
      "@id": "indimp:userType",
      "@type": "rdf:Property",
      "skos:definition": "The Independent Impact platform user type.",
      "rdfs:label": "userType",
      "schema:domainIncludes": {
        "@id": "indimp:PlatformUser"
      },
      "schema:rangeIncludes": {
        "@id": "schema:Text"
      }
    },
	{
 	  "@id": "indimp:userTypeShape",
	  "@type": "sh:NodeShape",
	  "sh:targetClass": { "@id": "indimp:PlatformUser" },
	  "sh:property": {
		"sh:path": { "@id": "indimp:userType" },
		"sh:datatype": { "@id": "xsd:string" },
		"sh:in": [ "STANDARD_REGISTRY", "USER" ],
		"sh:minCount": 1,
		"sh:maxCount": 1
	  }
	},
	{
      "@id": "indimp:dateRegistered",
      "@type": "rdf:Property",
      "skos:definition": "The timestamp at which a user account was created on the Independent Impact platform.",
      "rdfs:label": "dateRegistered",
      "schema:domainIncludes": {
        "@id": "indimp:PlatformUser"
      },
      "schema:rangeIncludes": {
        "@id": "schema:DateTime"
      }
    },
	{
      "@id": "indimp:didDocument",
      "@type": "rdf:Property",
      "skos:definition": "The document providing a platform user's DID and its associated properties.",
      "rdfs:label": "didDocument",
      "schema:domainIncludes": {
        "@id": "indimp:PlatformUser"
      },
      "schema:rangeIncludes": {
        "@id": "data:Document"
      }
    },
	
    {
      "@id": "indimp:AgentLicense",
	  "@type": "rdfs:Class",
	  "skos:definition": "A license that allows a platform user to perform specialised actions on the Independent Impact platform.",
      "rdfs:label": "AgentLicense",
      "rdfs:subClassOf": {
        "@id": "vcdm:VerifiableCredential"
      }
    },
	{
      "@id": "indimp:licenseNumber",
      "@type": "rdf:Property",
      "skos:definition": "A unique string identifier for an Independent Impact Agent License.",
      "rdfs:label": "licenseNumber",
      "schema:domainIncludes": {
        "@id": "indimp:AgentLicense"
      },
      "schema:rangeIncludes": {
        "@id": "schema:Text"
      }
    },
	{
	  "@id": "indimp:LicenseNumberShape",
	  "@type": "sh:NodeShape",
	  "sh:targetClass": { "@id": "indimp:AgentLicense" },
	  "sh:property": {
		"sh:path": { "@id": "indimp:licenseNumber" },
		"sh:datatype": { "@id": "xsd:string" },
		"sh:pattern": "^II-(PD|PV|MV)-[0-9]{2}X[0-9]{2}X[0-9]{11}-[0-9]{8}$",
		"sh:minCount": 1,
		"sh:maxCount": 1
	  }
	},	
	{
      "@id": "indimp:licenseScope",
      "@type": "rdf:Property",
      "skos:definition": "The label of the set of actions that the holder of the license is allowed to perform on the Independent Impact platform.",
      "rdfs:label": "licenseScope",
      "schema:domainIncludes": {
        "@id": "indimp:AgentLicense"
      },
      "schema:rangeIncludes": {
        "@id": "schema:Text"
      }
    },
	{
 	  "@id": "indimp:licenseScopeShape",
	  "@type": "sh:NodeShape",
	  "sh:targetClass": { "@id": "indimp:AgentLicense" },
	  "sh:property": {
		"sh:path": { "@id": "indimp:licenseScope" },
		"sh:datatype": { "@id": "xsd:string" },
		"sh:in": [ "PROJECT_DEVELOPER", "PDD_VALIDATOR", "MR_VERIFIER" ],
		"sh:minCount": 1,
		"sh:maxCount": 1
	  }
	},	
	{
      "@id": "indimp:hasAgentLicense",
      "@type": "rdf:Property",
      "skos:definition": "An Independent Impact Agent License held by a platform user.",
      "rdfs:label": "hasAgentLicense",
      "schema:domainIncludes": {
        "@id": "indimp:PlatformUser"
      },
      "schema:rangeIncludes": {
        "@id": "indimp:AgentLicense"
      }
    },	
	
	{
      "@id": "indimp:resourceHederaMessageId",
      "@type": "rdf:Property",
      "skos:definition": "The ID of the Hedera consensus message that recorded the moment of publication, listing or receipt (by the II platform) of the resource in question.",
      "rdfs:label": "hederaMessageId",
      "schema:domainIncludes": {
        "@id": "dcterms:Resource"
      },
      "schema:rangeIncludes": {
        "@id": "hed:HederaMessageId"
      }
    },
	{
      "@id": "indimp:resourceIpfsUri",
      "@type": "rdf:Property",
      "skos:definition": "The IPFS URI, if any, of the resource in question.",
      "rdfs:label": "ipfsUri",
      "schema:domainIncludes": {
        "@id": "dcterms:Resource"
      },
      "schema:rangeIncludes": {
        "@id": "schema:Text"
      },
	  "rdfs:comment": "If no value is provided for this property, the content of the resource should be provided via the data:resourceContent property, or the location of the content should be provided via the data:resourceContentLocation property."
    },
	{
	  "@id": "indimp:resourceIpfsUriShape",
	  "@type": "sh:NodeShape",
	  "sh:targetClass": { "@id": "dcterms:Resource" },
	  "sh:property": {
		"sh:path": { "@id": "indimp:resourceIpfsUri" },
		"sh:datatype": { "@id": "xsd:string" },
		"sh:pattern": "^(ipfs|ipns):\/\/[a-zA-Z0-9]+(?:\/[a-zA-Z0-9\/._-]*)?$",
		"sh:minCount": 1,
		"sh:maxCount": 1
	  }
	},
	{
      "@id": "indimp:documentSchema",
      "@type": "rdf:Property",
      "skos:definition": "A schema specifying the format and structure that a document must adhere to.",
      "rdfs:label": "documentSchema",
      "schema:domainIncludes": {
        "@id": "data:Document"
      },
      "schema:rangeIncludes": {
        "@id": "indimp:DocumentSchema"
      }
    },
	{
      "@id": "indimp:isEncrypted",
      "@type": "rdf:Property",
      "skos:definition": "Indicates whether the content of a resource is encrypted.",
      "rdfs:label": "isEncrypted",
      "schema:domainIncludes": {
        "@id": "dcterms:Resource"
      },
      "schema:rangeIncludes": {
        "@id": "schema:Boolean"
      }
    },
	{
      "@id": "indimp:documentAuthor",
      "@type": "rdf:Property",
      "skos:definition": "Identifies an entity responsible for the creation of the content of a document.",
      "rdfs:label": "author",
      "schema:domainIncludes": {
        "@id": "data:Document"
      },
      "schema:rangeIncludes": [
		{ "@id": "indimp:PlatformUser" },
		{ "@id": "aiao:Agent" },
		{ "@id": "schema:Text" }
	  ]
    },
	{
      "@id": "indimp:authProof",
      "@type": "rdf:Property",
      "skos:definition": "The mechanism by which the authenticity of a document can be proven.",
      "rdfs:label": "authProof",
      "schema:domainIncludes": {
        "@id": "data:Document"
      },
      "schema:rangeIncludes": {
        "@id": "schema:Text"
      }
    },
	{
 	  "@id": "indimp:authProofShape",
	  "@type": "sh:NodeShape",
	  "sh:targetClass": { "@id": "data:Document" },
	  "sh:property": {
		"sh:path": { "@id": "indimp:authProof" },
		"sh:datatype": { "@id": "xsd:string" },
		"sh:in": [ "NONE", "RSA_SIGNATURE", "VC" ],
		"sh:minCount": 1,
		"sh:maxCount": 1
	  }
	},
	
	{
      "@id": "indimp:Workflow",
	  "@type": "rdfs:Class",
	  "rdfs:comment": "A set of actions, processes or procedures that must be executed or performed to achieve a specific outcome.",
      "rdfs:label": "Workflow",
      "rdfs:subClassOf": {
        "@id": "aiao:Control"
      }
    },
	{
      "@id": "indimp:WorkflowStep",
	  "@type": "rdfs:Class",
	  "rdfs:comment": "A single action, process or procedure of a workflow.",
      "rdfs:label": "WorkflowStep",
      "rdfs:subClassOf": {
        "@id": "aiao:Control"
      }
    },
	{
      "@id": "indimp:hasWorkflowStep",
	  "@type": "rdf:Property",
	  "rdfs:comment": "A specific step of a workflow.",
      "rdfs:label": "Workflow",
      "schema:domainIncludes": {
        "@id": "indimp:Workflow"
      },
      "schema:rangeIncludes": {
        "@id": "indimp:WorkflowStep"
      }
    },
	
	{
      "@id": "indimp:WorkflowDocumentSubmission",
	  "@type": "rdfs:Class",
	  "rdfs:comment": "Records the submission of a document to a specific step of a specific workflow for a specific workflow subject.",
      "rdfs:label": "WorkflowDocumentSubmission",
      "rdfs:subClassOf": {
        "@id": "owl:Thing"
      }
    },
	{
      "@id": "indimp:workflow",
	  "@type": "rdf:Property",
	  "rdfs:comment": "The workflow to which a document was submitted, or in the context of which an agent-activity relation exists.",
      "rdfs:label": "workflow",
      "schema:domainIncludes": [
	    { "@id": "indimp:WorkflowDocumentSubmission" },
        { "@id": "indimp:AgentActivityWorkflowRelation" }
	  ],
      "schema:rangeIncludes": {
        "@id": "indimp:Workflow"
      }
    },
	{
      "@id": "indimp:workflowStep",
	  "@type": "rdf:Property",
	  "rdfs:comment": "The workflow step to which the document was submitted.",
      "rdfs:label": "workflowStep",
      "schema:domainIncludes": {
        "@id": "indimp:WorkflowDocumentSubmission"
      },
      "schema:rangeIncludes": {
        "@id": "indimp:WorkflowStep"
      }
    },
	{
      "@id": "indimp:workflowSubject",
	  "@type": "rdf:Property",
	  "rdfs:comment": "The subject of the workflow in respect of which or whom the document was submitted.",
      "rdfs:label": "workflowSubject",
      "schema:domainIncludes": {
        "@id": "indimp:WorkflowDocumentSubmission"
      },
      "schema:rangeIncludes": {
        "@id": "owl:Thing"
      }
    },
	{
      "@id": "indimp:workflowDocumentSubmittedBy",
	  "@type": "rdf:Property",
	  "rdfs:comment": "The platform user who submitted the document.",
      "rdfs:label": "submittedBy",
      "schema:domainIncludes": {
        "@id": "indimp:WorkflowDocumentSubmission"
      },
      "schema:rangeIncludes": {
        "@id": "indimp:PlatformUser"
      }
    },
	{
      "@id": "indimp:workflowDocumentSubmissionHederaMessageId",
      "@type": "rdf:Property",
      "skos:definition": "The ID of the Hedera consensus message that recorded the moment that a document was submitted to a specific workflow.",
      "rdfs:label": "hederaMessageId",
      "schema:domainIncludes": {
        "@id": "indimp:WorkflowDocumentSubmission"
      },
      "schema:rangeIncludes": {
        "@id": "hed:HederaMessageId"
      }
    },
	{
      "@id": "indimp:hasWorkflowSubmission",
	  "@type": "rdf:Property",
	  "rdfs:comment": "Provides details about a workflow submission for the document in question.",
      "rdfs:label": "hasWorkflowSubmission",
      "schema:domainIncludes": {
        "@id": "data:Document"
      },
      "schema:rangeIncludes": {
        "@id": "indimp:WorkflowDocumentSubmission"
      }
    },
	
	{
      "@id": "indimp:PlatformUserXhederaAccountLink",
	  "@type": "rdfs:Class",
	  "skos:definition": "Links an Independent Impact platform user to a Hedera account.",
      "rdfs:label": "PlatformUserXhederaAccountLink",
      "rdfs:subClassOf": {
        "@id": "owl:Thing"
      }
    },
	{
      "@id": "indimp:hederaAccount",
	  "@type": "rdf:Property",
	  "skos:definition": "A Hedera account.",
      "rdfs:label": "hederaAccount",
      "schema:domainIncludes": {
        "@id": "indimp:PlatformUserXhederaAccountLink"
      },
      "schema:rangeIncludes": {
        "@id": "hed:HederaAccount"
      }
    },
	{
      "@id": "indimp:platformUserXhederaAccountLinkDescription",
	  "@type": "rdf:Property",
	  "skos:definition": "A description of the link between a platform user and a Hedera account, e.g., 'PRIMARY_ACCOUNT'.",
      "rdfs:label": "description",
      "schema:domainIncludes": {
        "@id": "indimp:PlatformUserXhederaAccountLink"
      },
      "schema:rangeIncludes": {
        "@id": "schema:Text"
      }
    },
	
	{
      "@id": "indimp:isLinkedToHederaAccount",
	  "@type": "rdf:Property",
	  "rdfs:comment": "Links an Independent Impact platform user to a Hedera account.",
      "rdfs:label": "isLinkedToHederaAccount",
      "schema:domainIncludes": {
        "@id": "indimp:PlatformUser"
      },
      "schema:rangeIncludes": {
        "@id": "indimp:PlatformUserXhederaAccountLink"
      }
    },
	
	{
      "@id": "indimp:EntityXhederaTopicLink",
	  "@type": "rdfs:Class",
	  "skos:definition": "Links an Independent Impact entity (user, project, methodology, etc.) to a Hedera topic.",
      "rdfs:label": "EntityXhederaTopicLink",
      "rdfs:subClassOf": {
        "@id": "owl:Thing"
      }
    },
	{
      "@id": "indimp:hederaTopic",
	  "@type": "rdf:Property",
	  "skos:definition": "A Hedera topic.",
      "rdfs:label": "hederaTopic",
      "schema:domainIncludes": {
        "@id": "indimp:EntityXhederaTopicLink"
      },
      "schema:rangeIncludes": {
        "@id": "hed:HederaTopic"
      }
    },
	{
      "@id": "indimp:entityXhederaTopicLinkDescription",
	  "@type": "rdf:Property",
	  "skos:definition": "A description of the link between an entity and a Hedera topic, e.g., 'DID'.",
      "rdfs:label": "description",
      "schema:domainIncludes": {
        "@id": "indimp:EntityXhederaTopicLink"
      },
      "schema:rangeIncludes": {
        "@id": "schema:Text"
      }
    },

	{
      "@id": "indimp:isLinkedToHederaTopic",
	  "@type": "rdf:Property",
	  "rdfs:comment": "Links an Independent Impact entity to a Hedera topic.",
      "rdfs:label": "isLinkedToHederaTopic",
      "schema:domainIncludes": {
        "@id": "indimp:PlatformUser"
      },
      "schema:rangeIncludes": {
        "@id": "indimp:EntityXhederaTopicLink"
      }
    },

	{
      "@id": "indimp:isReviewOf",
	  "@type": "rdf:Property",
	  "rdfs:comment": "Identifies a document as a review of another document.",
      "rdfs:label": "isReviewOf",
      "schema:domainIncludes": {
        "@id": "data:Document"
      },
      "schema:rangeIncludes": {
        "@id": "data:Document"
      }
    },
	
	{
      "@id": "indimp:AgentActivityWorkflowRelation",
	  "@type": "rdfs:Class",
	  "skos:definition": "Relates an agent to an activity in the context of a specific workflow.",
      "rdfs:label": "AgentActivityWorkflowRelation",
      "rdfs:subClassOf": {
        "@id": "aiao:AgentActivityRelation"
      }
    },
	
	{
      "@id": "indimp:dateCreated",
      "@type": "rdf:Property",
      "skos:definition": "The timestamp at which a project was created on the Independent Impact platform.",
      "rdfs:label": "dateCreated",
      "schema:domainIncludes": {
        "@id": "aiao:Project"
      },
      "schema:rangeIncludes": {
        "@id": "schema:DateTime"
      }
    },
	{
      "@id": "indimp:createdBy",
      "@type": "rdf:Property",
      "skos:definition": "The Independent Impact platform user who created the project.",
      "rdfs:label": "createdBy",
      "schema:domainIncludes": {
        "@id": "aiao:Project"
      },
      "schema:rangeIncludes": {
        "@id": "indimp:PlatformUser"
      }
    },
	{
      "@id": "indimp:title",
      "@type": "rdf:Property",
      "skos:definition": "A human-friendly title for an activity or project.",
      "rdfs:label": "title",
      "schema:domainIncludes": [
		{ "@id": "aiao:Activity" },
		{ "@id": "aiao:Project" }
	  ],
      "schema:rangeIncludes": {
        "@id": "schema:Text"
      }
    },
	
	{
      "@id": "indimp:DocumentSchema",
	  "@type": "rdfs:Class",
	  "skos:definition": "A specification for the structure and data types of a document.",
      "rdfs:label": "DocumentSchema",
      "rdfs:subClassOf": [
		{ "@id": "dcterms:Resource" },
		{ "@id": "aiao:Control" }
	  ]
    }
  ]
}